untimed/NewSpfStep.thy
@@ -394,7 +394,7 @@ qed
 lemma sbElem_surj:"\<exists>sb. sbE =  Abs_sbElem (inv convDiscrUp (sbHdElem\<cdot>sb)) \<and> sbHdElemWell sb"
   sorry
     
-lemma spfStep_inj_on:"inj_on (Rep_cfun (spfStep_inj In Out)) {h. \<forall>m. ufDom\<cdot>(h m) = In \<and> ufRan\<cdot>(h m) = Out}"
+lemma spfStep_inj_on[simp]:"inj_on (Rep_cfun (spfStep_inj In Out)) {h. \<forall>m. ufDom\<cdot>(h m) = In \<and> ufRan\<cdot>(h m) = Out}"
 proof(simp add: spfStep_inj_def, rule inj_onI)
   fix x y :: "'a sbElem \<Rightarrow> ('a stream\<^sup>\<Omega>) ufun"
   assume ax:" x \<in> {h. \<forall>m. ufDom\<cdot>(h m) = In \<and> ufRan\<cdot>(h m) = Out}"
